LeanPy/Data/Object/TypeRef.lean
@@ -4,6 +4,7 @@ Released under the Apache 2.0 license as described in the file LICENSE.
 Authors: Mac Malone
 -/
 import LeanPy.Data.Type.Init
+import LeanPy.Data.Type.Mro
 
 namespace LeanPy
 
@@ -18,6 +19,16 @@ def objectType.doc : String := "\
   name := "object"
   doc? := some objectType.doc
 
-initialize objectTypeRef.init : InitTypeRef objectType ← initTypeRef
+@[simp] theorem baseMro_objectType :
+  objectType.baseMro = []
+:= rfl
 
-abbrev objectTypeRef : TypeRef := objectTypeRef.init.toTypeRef
+private initialize objectTypeInitRef : InitTypeRef objectType ← initTypeRef
+
+@[inline] def objectTypeRawRef : RawTypeRef := objectTypeInitRef.toRawTypeRef
+
+@[simp] theorem isNonScalar_addr_objectTypeRawRef : objectTypeRawRef.addr.isNonScalar :=
+  objectTypeInitRef.isNonScalar_addr
+
+@[simp] theorem data_objectTypeRawRef : objectTypeRawRef.data = objectType :=
+  objectTypeInitRef.data_toRawTypeRef
