LeanPy/Data/Type/Lawful.lean
@@ -6,8 +6,8 @@ Authors: Mac Malone
 import LeanPy.Data.Type.Mro
 import LeanPy.Data.Type.TypeRef
 import LeanPy.Data.Object.TypeRef
-import LeanPy.Data.Bool.TypeRef
 import LeanPy.Data.Int.TypeRef
+import LeanPy.Data.Bool.TypeRef
 import LeanPy.Data.None.TypeRef
 import LeanPy.Data.Str.TypeRef
 import LeanPy.Data.Tuple.TypeRef
@@ -15,27 +15,37 @@ import LeanPy.Data.Dict.TypeRef
 
 namespace LeanPy
 
+abbrev objectTypeRef : TypeRef := ⟨objectTypeRawRef⟩
+abbrev typeTypeRef : TypeRef := ⟨typeTypeRawRef⟩
+abbrev intTypeRef : TypeRef := ⟨intTypeRawRef⟩
+abbrev boolTypeRef : TypeRef := ⟨boolTypeRawRef⟩
+abbrev noneTypeRef : TypeRef := ⟨noneTypeRawRef⟩
+abbrev strTypeRef : TypeRef := ⟨strTypeRawRef⟩
+abbrev tupleTypeRef : TypeRef := ⟨tupleTypeRawRef⟩
+abbrev dictTypeRef : TypeRef := ⟨dictTypeRawRef⟩
+
 /-! ## LawfulTypeRef -/
 
 class LawfulType (self : PyType) : Prop where
-  objectType_mem_baseMro : objectTypeRef ∈ self.baseMro
-  isTypeSubclass_iff :
-    self.isTypeSubclass ↔ self = typeTypeRef.data ∨ typeTypeRef ∈ self.baseMro
-  isIntSubclass_iff :
-    self.isIntSubclass ↔ self = intTypeRef.data ∨ intTypeRef ∈ self.baseMro
-  isStrSubclass_iff :
-    self.isStrSubclass ↔ self = strTypeRef.data ∨ strTypeRef ∈ self.baseMro
-  isTupleSubclass_iff :
-    self.isTupleSubclass ↔ self = tupleTypeRef.data ∨ tupleTypeRef ∈ self.baseMro
-  isDictSubclass_iff :
-    self.isDictSubclass ↔ self = dictTypeRef.data ∨ dictTypeRef ∈ self.baseMro
-  isValidObject_mro {id data} :
-    self.IsValidObject id data → ∀ {ty}, ty ∈ self.baseMro → ty.IsValidObject id data
+  eq_objectType_or_objectTypeRef_mem_baseMro :
+    self = objectType ∨ objectTypeRawRef ∈ self.baseMro := by simp
+  isTypeSubclass_iff : self.isTypeSubclass ↔
+    self = typeType ∨ typeTypeRawRef ∈ self.baseMro := by simp [FrozenRef.eq_iff]
+  isIntSubclass_iff : self.isIntSubclass ↔
+    self = intType ∨ intTypeRawRef ∈ self.baseMro := by simp [FrozenRef.eq_iff]
+  isStrSubclass_iff : self.isStrSubclass ↔
+    self = strType ∨ strTypeRawRef ∈ self.baseMro := by simp [FrozenRef.eq_iff]
+  isTupleSubclass_iff : self.isTupleSubclass ↔
+    self = tupleType ∨ tupleTypeRawRef ∈ self.baseMro := by simp [FrozenRef.eq_iff]
+  isDictSubclass_iff : self.isDictSubclass ↔
+    self = dictType ∨ dictTypeRawRef ∈ self.baseMro := by simp [FrozenRef.eq_iff]
+  isValidObject_mro {id data} : self.IsValidObject id data →
+    ∀ {ty}, ty ∈ self.baseMro → ty.data.IsValidObject id data := by simp
 
 namespace PyType
 
 export LawfulType (
-  objectType_mem_baseMro
+  eq_objectType_or_objectTypeRef_mem_baseMro
   isIntSubclass_iff isTypeSubclass_iff isStrSubclass_iff
   isTupleSubclass_iff isDictSubclass_iff
   isValidObject_mro
@@ -58,13 +68,13 @@ class LawfulTypeRef (self : TypeRef) : Prop where
       simp [TypeRef.Subtype.iff_mem_mro, TypeRef.mem_mro_iff, TypeRef.eq_iff]
   isTupleSubclass_iff_subset :
     self.isTupleSubclass ↔ self ⊆ tupleTypeRef := by
-      simp [TypeRef.Subtype.iff_mem_mro, TypeRef.mro_eq_cons_baseMro, TypeRef.eq_iff]
+      simp [TypeRef.Subtype.iff_mem_mro, TypeRef.mro_eq_cons, TypeRef.eq_iff]
   isDictSubclass_iff_subset :
     self.isDictSubclass ↔ self ⊆ dictTypeRef := by
-      simp [TypeRef.Subtype.iff_mem_mro, TypeRef.mro_eq_cons_baseMro, TypeRef.eq_iff]
+      simp [TypeRef.Subtype.iff_mem_mro, TypeRef.mro_eq_cons, TypeRef.eq_iff]
   isValidObject_mro {id data} :
     self.IsValidObject id data → ∀ {ty}, self ⊆ ty → ty.IsValidObject id data
-  := by simp_all [TypeRef.Subtype.iff_mem_mro, TypeRef.mro_eq_cons_baseMro]
+  := by simp_all [TypeRef.Subtype.iff_mem_mro, TypeRef.mro_eq_cons]
 
 namespace TypeRef
 
@@ -83,53 +93,45 @@ abbrev id (self : TypeRef) [LawfulTypeRef self] : ObjectId :=
 
 end TypeRef
 
-@[simp] theorem data_objectTypeRef : objectTypeRef.data = objectType := rfl
-
-@[simp] theorem mro_objectTypeRef :
+@[simp] theorem baseMro_objectTypeRef :
   objectTypeRef.baseMro = []
 := rfl
-
-@[simp] theorem data_typeTypeRef : typeTypeRef.data = typeType := rfl
 
 @[simp] theorem baseMro_typeTypeRef :
   typeTypeRef.baseMro = [objectTypeRef]
 := rfl
 
-@[simp] theorem data_noneTypeRef : noneTypeRef.data = noneType := rfl
-
 @[simp] theorem baseMro_noneTypeRef :
   noneTypeRef.baseMro = [objectTypeRef]
 := rfl
-
-@[simp] theorem data_strTypeRef : strTypeRef.data = strType := rfl
 
 @[simp] theorem baseMro_strTypeRef :
   strTypeRef.baseMro = [objectTypeRef]
 := rfl
 
-@[simp] theorem data_tupleTypeRef : tupleTypeRef.data = tupleType := rfl
-
 @[simp] theorem baseMro_tupleTypeRef :
   tupleTypeRef.baseMro = [objectTypeRef]
 := rfl
-
-@[simp] theorem data_dictTypeRef : dictTypeRef.data = dictType := rfl
 
 @[simp] theorem baseMro_dictTypeRef :
   dictTypeRef.baseMro = [objectTypeRef]
 := rfl
 
-@[simp] theorem data_intTypeRef : intTypeRef.data = intType := rfl
-
 @[simp] theorem baseMro_intTypeRef :
   intTypeRef.baseMro = [objectTypeRef]
 := rfl
 
-@[simp] theorem data_boolTypeRef : boolTypeRef.data = boolType := rfl
-
 @[simp] theorem baseMro_boolTypeRef :
   boolTypeRef.baseMro = [intTypeRef, objectTypeRef]
 := rfl
+
+instance : LawfulType objectType where
+instance : LawfulType typeType where
+instance : LawfulType noneType where
+instance : LawfulType tupleType where
+instance : LawfulType dictType where
+instance : LawfulType intType where
+instance : LawfulType boolType where
 
 instance : LawfulTypeRef objectTypeRef where
 instance : LawfulTypeRef typeTypeRef where
@@ -145,45 +147,47 @@ theorem LawfulTypeRef.ofLawfulType {ty : TypeRef}
 : LawfulTypeRef ty where
   isNonScalar_addr := h_addr
   subset_objectType := by
-    grind [TypeRef.Subtype.iff_mem_mro, TypeRef.mro_eq_cons_baseMro,
-      TypeRef.baseMro_eq_data_baseMro, LawfulType.objectType_mem_baseMro]
+    grind [
+      TypeRef.Subtype.iff_mem_mro, TypeRef.mro_eq_cons,
+      TypeRef.mem_baseMro_iff_mem_data_baseMro,
+      LawfulType.eq_objectType_or_objectTypeRef_mem_baseMro]
   isTypeSubclass_iff_subset := by
     have data_ne : ty.data ≠ typeType := by
       match h:ty.data with | .mk .. => grind
     have ty_ne : typeTypeRef ≠ ty := TypeRef.ne_of_data_ne data_ne.symm
     simp [data_ne, ty_ne, TypeRef.Subtype.iff_mem_mro, TypeRef.mem_mro_iff,
-      LawfulType.isTypeSubclass_iff, TypeRef.baseMro_eq_data_baseMro]
+      LawfulType.isTypeSubclass_iff, TypeRef.mem_baseMro_iff_mem_data_baseMro]
   isIntSubclass_iff_subset := by
     have data_ne : ty.data ≠ intType := by
       match h:ty.data with | .mk .. => grind
     have ty_ne : intTypeRef ≠ ty := TypeRef.ne_of_data_ne data_ne.symm
     simp [data_ne, ty_ne, TypeRef.Subtype.iff_mem_mro, TypeRef.mem_mro_iff,
-      LawfulType.isIntSubclass_iff, TypeRef.baseMro_eq_data_baseMro]
+      LawfulType.isIntSubclass_iff, TypeRef.mem_baseMro_iff_mem_data_baseMro]
   isTupleSubclass_iff_subset := by
     have data_ne : ty.data ≠ tupleType := by
       match h:ty.data with | .mk .. => grind
     have ty_ne : tupleTypeRef ≠ ty := TypeRef.ne_of_data_ne data_ne.symm
     simp [data_ne, ty_ne, TypeRef.Subtype.iff_mem_mro, TypeRef.mem_mro_iff,
-      LawfulType.isTupleSubclass_iff, TypeRef.baseMro_eq_data_baseMro]
+      LawfulType.isTupleSubclass_iff, TypeRef.mem_baseMro_iff_mem_data_baseMro]
   isDictSubclass_iff_subset := by
     have data_ne : ty.data ≠ dictType := by
       match h:ty.data with | .mk .. => grind
     have ty_ne : dictTypeRef ≠ ty := TypeRef.ne_of_data_ne data_ne.symm
     simp [data_ne, ty_ne,TypeRef.Subtype.iff_mem_mro, TypeRef.mem_mro_iff,
-      LawfulType.isDictSubclass_iff, TypeRef.baseMro_eq_data_baseMro]
+      LawfulType.isDictSubclass_iff, TypeRef.mem_baseMro_iff_mem_data_baseMro]
   isStrSubclass_iff_subset := by
     have data_ne : ty.data ≠ strType := by
       match h:ty.data with | .mk .. => grind
     have ty_ne : strTypeRef ≠ ty := TypeRef.ne_of_data_ne data_ne.symm
-    simp [data_ne, ty_ne,TypeRef.Subtype.iff_mem_mro, TypeRef.mem_mro_iff,
-      LawfulType.isStrSubclass_iff, TypeRef.baseMro_eq_data_baseMro]
+    simp [data_ne, ty_ne, TypeRef.Subtype.iff_mem_mro, TypeRef.mem_mro_iff,
+      LawfulType.isStrSubclass_iff, TypeRef.mem_baseMro_iff_mem_data_baseMro]
   isValidObject_mro := by
     intro id data
     simp only [
       TypeRef.IsValidObject,
       TypeRef.Subtype.iff_mem_mro, TypeRef.mem_mro_iff,
-      TypeRef.baseMro_eq_data_baseMro, forall_eq_or_imp]
+      TypeRef.mem_baseMro_iff_mem_data_baseMro, forall_eq_or_imp]
     intro h
     apply And.intro h
-    apply LawfulType.isValidObject_mro
-    exact h
+    intro _ h_mem
+    exact ty.data.isValidObject_mro h h_mem
